Work on label typing

.Makefile.d
@@ -4,6 +4,9 @@ CpdtTactics.vos CpdtTactics.vok CpdtTactics.required_vos: CpdtTactics.v
 Maps.vo Maps.glob Maps.v.beautified Maps.required_vo: Maps.v 
 Maps.vio: Maps.v 
 Maps.vos Maps.vok Maps.required_vos: Maps.v 
+NMaps.vo NMaps.glob NMaps.v.beautified NMaps.required_vo: NMaps.v 
+NMaps.vio: NMaps.v 
+NMaps.vos NMaps.vok NMaps.required_vos: NMaps.v 
 ourlang.vo ourlang.glob ourlang.v.beautified ourlang.required_vo: ourlang.v gh/CpdtTactics.vo Maps.vo
 ourlang.vio: ourlang.v gh/CpdtTactics.vio Maps.vio
 ourlang.vos ourlang.vok ourlang.required_vos: ourlang.v gh/CpdtTactics.vos Maps.vos
